work on bir_program_termination theory
extend this theory and reason properly what happend, if a program
terminates

src/core-props/bir_program_terminationScript.sml
@@ -1,6 +1,7 @@
 open HolKernel Parse boolLib bossLib;
 open bir_programTheory bir_program_valid_stateTheory HolBACoreSimps;
-
+open bir_program_multistep_propsTheory bir_auxiliaryTheory
+open bir_valuesTheory bir_immTheory
 
 val _ = new_theory "bir_program_termination";
 
@@ -10,43 +11,49 @@ val _ = new_theory "bir_program_termination";
 (* program to terminate                                                      *)
 (* ------------------------------------------------------------------------- *)
 
-(* TODO: extend this significantly *)
 
+(***************************************)
+(* Termination changes just the status *)
+(***************************************)
 
-val bir_exec_stmtB_not_halted_jumped = store_thm ("bir_exec_stmtB_not_halted_jumped",
-``(!st stmt l. (st.bst_status <> BST_JumpOutside l) ==> ((bir_exec_stmtB_state stmt st).bst_status <> BST_JumpOutside l)) /\
-  (!st stmt v. (st.bst_status <> BST_Halted v) ==> ((bir_exec_stmtB_state stmt st).bst_status <> BST_Halted v))``,
+(* If we are in a non-terminated state, execute a statement and
+   terminate, then only the status was changed. Otherwise the state
+   stays unchanged, including the PC and all the values. This means
+   that we can easily examine which statement went wrong. *)
 
-CONJ_TAC >> Cases_on `stmt` >> (
-  ASM_SIMP_TAC std_ss [bir_exec_stmtB_state_REWRS, LET_DEF,
-    bir_exec_stmt_declare_def, bir_exec_stmt_assume_def,
-    bir_exec_stmt_assign_def, bir_exec_stmt_assert_def,
-    bir_exec_stmt_observe_state_def] >>
-  REPEAT GEN_TAC >> STRIP_TAC >>
-  REPEAT CASE_TAC >>
-  FULL_SIMP_TAC (std_ss++holBACore_ss) [bir_state_set_failed_def]
-));
-
-
+(* The property holds for basic statements *)
 val bir_exec_stmtB_terminates_no_change = store_thm ("bir_exec_stmtB_terminates_no_change",
-``!st stmt. ~(bir_state_is_terminated st) ==>
-              (bir_state_is_terminated (bir_exec_stmtB_state stmt st)) ==>
-              (((bir_exec_stmtB_state stmt st) with bst_status := BST_Running) = st)``,
+``!st stmt fe st'.
+     ~(bir_state_is_terminated st) ==>
+     (bir_exec_stmtB stmt st = (fe, st')) ==>
+     (bir_state_is_terminated st') ==>
+     (((st' with bst_status := BST_Running) = st) /\ (fe = NONE))``,
 
 SIMP_TAC (std_ss++holBACore_ss) [bir_state_is_terminated_def,
   bir_state_t_component_equality, bir_exec_stmtB_pc_unchanged] >>
 Cases_on `stmt` >> (
-  SIMP_TAC std_ss [bir_exec_stmtB_state_REWRS, LET_DEF,
+  SIMP_TAC std_ss [bir_exec_stmtB_def, LET_DEF,
     bir_exec_stmt_declare_def, bir_exec_stmt_assume_def,
     bir_exec_stmt_assign_def, bir_exec_stmt_assert_def,
-    bir_exec_stmt_observe_state_def] >>
+    bir_exec_stmt_observe_def] >>
   REPEAT GEN_TAC >> STRIP_TAC >>
   REPEAT CASE_TAC >>
   FULL_SIMP_TAC (std_ss++holBACore_ss) [bir_state_set_failed_def,
-    bir_state_is_terminated_def]
+    bir_state_is_terminated_def, bir_state_t_component_equality]
 ));
 
+val bir_exec_stmtB_terminates_no_change_state = store_thm ("bir_exec_stmtB_terminates_no_change_state",
+``!st stmt. ~(bir_state_is_terminated st) ==>
+              (bir_state_is_terminated (bir_exec_stmtB_state stmt st)) ==>
+              (((bir_exec_stmtB_state stmt st) with bst_status := BST_Running) = st)``,
 
+REPEAT STRIP_TAC >>
+Cases_on `bir_exec_stmtB stmt st` >>
+FULL_SIMP_TAC std_ss [bir_exec_stmtB_state_def] >>
+METIS_TAC[bir_exec_stmtB_terminates_no_change]);
+
+
+(* And for end statements *)
 val bir_exec_stmtE_terminates_no_change = store_thm ("bir_exec_stmtE_terminates_no_change",
 ``!p st stmt. ~(bir_state_is_terminated st) ==>
               (bir_state_is_terminated (bir_exec_stmtE p stmt st)) ==>
@@ -61,6 +68,343 @@ Cases_on `stmt` >> (
   REPEAT CASE_TAC >>
   FULL_SIMP_TAC (std_ss++holBACore_ss) [bir_state_set_failed_def]
 ));
+
+
+(* Thus it holds for all statements. *)
+val bir_exec_stmt_terminates_no_change = store_thm ("bir_exec_stmt_terminates_no_change",
+``!p st (stmt:'a bir_stmt_t) fe st'. ~(bir_state_is_terminated st) ==>
+              (bir_exec_stmt p stmt st = (fe, st')) ==>
+              (bir_state_is_terminated st') ==>
+              (((st' with bst_status := BST_Running) = st) /\ (fe = NONE))``,
+
+Cases_on `stmt:'a bir_stmt_t` >| [
+  REPEAT GEN_TAC >> REPEAT DISCH_TAC >>
+  rename1 `BStmtB (stmtB:'a bir_stmt_basic_t)` >>
+  MP_TAC (Q.SPECL [`st`, `stmtB:'a bir_stmt_basic_t`] bir_exec_stmtB_terminates_no_change) >>
+  `?fe' st''. bir_exec_stmtB stmtB st = (fe', st'')` by METIS_TAC[pairTheory.PAIR] >>
+  ASM_SIMP_TAC std_ss [] >>
+  Cases_on `st''.bst_status = BST_Running` >> (
+    FULL_SIMP_TAC (std_ss++holBACore_ss) [
+      bir_exec_stmt_def, LET_DEF, bir_state_is_terminated_def,
+      bir_state_t_component_equality]
+  ),
+
+  SIMP_TAC std_ss [bir_exec_stmt_def, bir_exec_stmtE_terminates_no_change]
+]);
+
+
+val bir_exec_stmt_terminates_no_change_state = store_thm ("bir_exec_stmt_terminates_no_change_state",
+``!p st (stmt:'a bir_stmt_t). ~(bir_state_is_terminated st) ==>
+              (bir_state_is_terminated (bir_exec_stmt_state p stmt st)) ==>
+             (((bir_exec_stmt_state p stmt st) with bst_status := BST_Running) = st)``,
+
+REPEAT STRIP_TAC >>
+Cases_on `bir_exec_stmt p stmt st` >>
+FULL_SIMP_TAC std_ss [bir_exec_stmt_state_def] >>
+METIS_TAC[bir_exec_stmt_terminates_no_change]);
+
+
+(* It holds for single steps *)
+val bir_exec_step_terminates_no_change = store_thm ("bir_exec_step_terminates_no_change",
+``!p st fe st'. ~(bir_state_is_terminated st) ==>
+              (bir_exec_step p st = (fe, st')) ==>
+              (bir_state_is_terminated st') ==>
+              (((st' with bst_status := BST_Running) = st) /\ (fe = NONE))``,
+
+SIMP_TAC std_ss [bir_exec_step_def] >>
+REPEAT GEN_TAC >> REPEAT DISCH_TAC >>
+Cases_on `bir_get_current_statement p st.bst_pc` >| [
+  FULL_SIMP_TAC (std_ss++holBACore_ss) [bir_state_set_failed_def, bir_state_is_terminated_def,
+    bir_state_t_component_equality],
+
+  FULL_SIMP_TAC std_ss [] >>
+  METIS_TAC[bir_exec_stmt_terminates_no_change]
+]);
+
+
+val bir_exec_step_terminates_no_change_state = store_thm (
+"bir_exec_step_terminates_no_change_state",
+``!p st. ~(bir_state_is_terminated st) ==>
+         (bir_state_is_terminated (bir_exec_step_state p st)) ==>
+         (((bir_exec_step_state p st) with bst_status := BST_Running) = st)``,
+
+REPEAT STRIP_TAC >>
+Cases_on `bir_exec_step p st` >>
+FULL_SIMP_TAC std_ss [bir_exec_step_state_def] >>
+METIS_TAC[bir_exec_step_terminates_no_change]);
+
+
+
+(* We can iterate with same effect *)
+val bir_exec_step_n_last_step_terminates = store_thm ("bir_exec_step_n_last_step_terminates",
+``!p st st' l i n.
+     ~(bir_state_is_terminated st) ==>
+     (bir_exec_step_n p st n = (l, SUC i, st')) ==>
+     (bir_state_is_terminated st') ==> (
+     ?st''. (bir_exec_step_n p st i = (l, i, st'')) /\
+            (st'' = st' with bst_status := BST_Running) /\
+            (bir_exec_step p st'' = (NONE, st')))``,
+
+REPEAT STRIP_TAC >>
+`bir_exec_step_n p st (SUC i) = (l, SUC i, st')` by METIS_TAC[bir_exec_steps_LIMIT_STEP_NO] >>
+`(?l' c' st''. bir_exec_step_n p st i = (l', c', st''))` by
+  METIS_TAC[pairTheory.PAIR] >>
+`c' <= i` by FULL_SIMP_TAC std_ss [bir_exec_step_n_EQ_THM] >>
+FULL_SIMP_TAC std_ss [bir_exec_step_n_SUC_END, LET_DEF] >>
+Cases_on `bir_state_is_terminated st''` >> (
+  FULL_SIMP_TAC arith_ss []
+) >>
+`?fe st'''. bir_exec_step p st'' = (fe, st''')` by
+  METIS_TAC[pairTheory.PAIR] >>
+FULL_SIMP_TAC std_ss [] >>
+REPEAT BasicProvers.VAR_EQ_TAC >>
+`(fe = NONE) /\ (st'' = (st' with bst_status := BST_Running))` by
+  METIS_TAC[bir_exec_step_terminates_no_change] >>
+FULL_SIMP_TAC list_ss [OPT_CONS_REWRS]);
+
+
+
+
+(*****************)
+(* Status Halted *)
+(*****************)
+
+val bir_exec_stmtB_status_not_halted = store_thm ("bir_exec_stmtB_status_not_halted",
+``!st stmt v. (st.bst_status <> BST_Halted v) ==> (((bir_exec_stmtB_state stmt st).bst_status <> BST_Halted v))``,
+
+Cases_on `stmt` >> (
+  ASM_SIMP_TAC (std_ss++holBACore_ss) [bir_exec_stmtB_state_REWRS, LET_DEF,
+    bir_exec_stmt_declare_def, bir_exec_stmt_assume_def,
+    bir_exec_stmt_assign_def, bir_exec_stmt_assert_def,
+    bir_exec_stmt_observe_state_def, bir_state_set_failed_def] >>
+  REPEAT GEN_TAC >>
+  REPEAT CASE_TAC >>
+  FULL_SIMP_TAC (std_ss++holBACore_ss) []
+));
+
+
+val bir_exec_stmtE_status_halted = store_thm ("bir_exec_stmtE_status_halted",
+``!st p stmt v. (st.bst_status <> BST_Halted v) ==> (((bir_exec_stmtE p stmt st).bst_status = BST_Halted v)) ==> (?e. (stmt = BStmt_Halt e) /\ (v = bir_eval_exp e st.bst_environ))``,
+
+Cases_on `stmt` >> (
+  ASM_SIMP_TAC (std_ss++holBACore_ss) [bir_exec_stmtE_def,
+    bir_exec_stmt_jmp_def, bir_state_set_failed_def, bir_exec_stmt_jmp_to_label_def,
+    bir_exec_stmt_cjmp_def, bir_exec_stmt_halt_def] >>
+  REPEAT GEN_TAC >>
+  REPEAT CASE_TAC >>
+  FULL_SIMP_TAC (std_ss++holBACore_ss) []
+));
+
+
+
+val bir_exec_stmt_status_halted = store_thm ("bir_exec_stmt_status_halted",
+``!st p stmt v. (st.bst_status <> BST_Halted v) ==> (((bir_exec_stmt_state p stmt st).bst_status = BST_Halted v)) ==> (?e. (stmt = BStmtE (BStmt_Halt e)) /\ (v = bir_eval_exp e st.bst_environ))``,
+
+Cases_on `stmt` >| [
+  SIMP_TAC (std_ss++boolSimps.LIFT_COND_ss++holBACore_ss) [bir_exec_stmt_state_REWRS, LET_DEF] >>
+  METIS_TAC[bir_exec_stmtB_status_not_halted],
+
+  SIMP_TAC (std_ss++holBACore_ss) [bir_exec_stmt_state_REWRS] >>
+  METIS_TAC[bir_exec_stmtE_status_halted]
+]);
+
+
+val bir_exec_step_status_halted = store_thm ("bir_exec_step_status_halted",
+``!st p v. (st.bst_status <> BST_Halted v) ==> (((bir_exec_step_state p st).bst_status = BST_Halted v)) ==> (?e. ((bir_get_current_statement p st.bst_pc = SOME (BStmtE (BStmt_Halt e)))) /\ (v = bir_eval_exp e st.bst_environ))``,
+
+REPEAT GEN_TAC >>
+SIMP_TAC (std_ss++boolSimps.LIFT_COND_ss) [bir_exec_step_state_def, bir_exec_step_def] >>
+CASE_TAC >> (
+  ASM_SIMP_TAC (std_ss++holBACore_ss) [bir_state_set_failed_def, GSYM bir_exec_stmt_state_def]
+) >>
+METIS_TAC[bir_exec_stmt_status_halted]);
+
+
+
+(**********************)
+(* Status JumpOutside *)
+(**********************)
+
+val bir_exec_stmtB_status_not_jumped = store_thm ("bir_exec_stmtB_status_not_jumped",
+``!st stmt l. (st.bst_status <> BST_JumpOutside l) ==> (((bir_exec_stmtB_state stmt st).bst_status <> BST_JumpOutside l))``,
+
+Cases_on `stmt` >> (
+  ASM_SIMP_TAC (std_ss++holBACore_ss) [bir_exec_stmtB_state_REWRS, LET_DEF,
+    bir_exec_stmt_declare_def, bir_exec_stmt_assume_def,
+    bir_exec_stmt_assign_def, bir_exec_stmt_assert_def,
+    bir_exec_stmt_observe_state_def, bir_state_set_failed_def] >>
+  REPEAT GEN_TAC >>
+  REPEAT CASE_TAC >>
+  FULL_SIMP_TAC (std_ss++holBACore_ss) []
+));
+
+
+val bir_stmtE_is_jmp_to_label_def = Define `bir_stmtE_is_jmp_to_label env l stmt <=>
+                ((?le. (stmt = BStmt_Jmp le) /\ (bir_eval_label_exp le env = SOME l)) \/
+                 (?le1 le2 ce c. (stmt = BStmt_CJmp ce le1 le2) /\
+                                 (bir_eval_exp ce env = BVal_Imm (bool2b c)) /\
+                                 (bir_eval_label_exp (if c then le1 else le2) env = SOME l)))`;
+
+val bir_stmtE_is_jmp_to_label_REWRS = store_thm ("bir_stmtE_is_jmp_to_label_REWRS",
+  ``(!le env l. (bir_stmtE_is_jmp_to_label env l (BStmt_Jmp le) <=>
+       (bir_eval_label_exp le env = SOME l))) /\
+    (!ce le1 le2 env l. (bir_stmtE_is_jmp_to_label env l (BStmt_CJmp ce le1 le2) <=>
+       case (bir_dest_bool_val (bir_eval_exp ce env)) of
+         | NONE => F
+         | SOME T => (bir_eval_label_exp le1 env = SOME l)
+         | SOME F => (bir_eval_label_exp le2 env = SOME l)
+    )) /\
+    (!l env e. (bir_stmtE_is_jmp_to_label env l (BStmt_Halt e) <=> F))``,
+
+SIMP_TAC (std_ss++holBACore_ss) [bir_stmtE_is_jmp_to_label_def] >>
+REPEAT GEN_TAC >> EQ_TAC >- (
+  STRIP_TAC >>
+  ASM_SIMP_TAC (std_ss++holBACore_ss) []  >>
+  METIS_TAC[]
+) >>
+REPEAT CASE_TAC >>
+FULL_SIMP_TAC (std_ss++holBACore_ss) [bir_dest_bool_val_EQ_SOME] >> METIS_TAC[]);
+
+
+val bir_stmtE_is_jmp_to_label_SEM = store_thm ("bir_stmtE_is_jmp_to_label_SEM",
+  ``!p stmt st l. (bir_stmtE_is_jmp_to_label st.bst_environ l stmt) ==>
+                  (bir_exec_stmtE p stmt st = bir_exec_stmt_jmp_to_label p l st)``,
+
+Cases_on `stmt` >>
+SIMP_TAC std_ss [bir_stmtE_is_jmp_to_label_REWRS, bir_exec_stmtE_def,
+  bir_exec_stmt_jmp_def, bir_exec_stmt_cjmp_def] >>
+REPEAT GEN_TAC >>
+REPEAT CASE_TAC);
+
+
+
+val bir_exec_stmtE_status_jumped = store_thm ("bir_exec_stmtE_status_jumped",
+``!st p stmt l. (st.bst_status <> BST_JumpOutside l) ==>
+                (((bir_exec_stmtE p stmt st).bst_status = BST_JumpOutside l)) ==>
+                ((~(MEM l (bir_labels_of_program p))) /\
+                 (bir_stmtE_is_jmp_to_label st.bst_environ l stmt))``,
+
+Cases_on `stmt` >> (
+  ASM_SIMP_TAC (std_ss++holBACore_ss) [bir_exec_stmtE_def,
+    bir_exec_stmt_jmp_def, bir_state_set_failed_def, bir_exec_stmt_jmp_to_label_def,
+    bir_exec_stmt_cjmp_def, bir_exec_stmt_halt_def, bir_stmtE_is_jmp_to_label_REWRS] >>
+  REPEAT GEN_TAC >>
+  REPEAT CASE_TAC >>
+  FULL_SIMP_TAC (std_ss++holBACore_ss) [] >>
+  METIS_TAC[]
+));
+
+
+val bir_stmt_is_jmp_to_label_def = Define `
+  (bir_stmt_is_jmp_to_label env l (BStmtB _) <=> F) /\
+  (bir_stmt_is_jmp_to_label env l (BStmtE stmt) = bir_stmtE_is_jmp_to_label env l stmt)`
+
+
+val bir_stmt_is_jmp_to_label_SEM = store_thm ("bir_stmt_is_jmp_to_label_SEM",
+  ``!p stmt st l. (bir_stmt_is_jmp_to_label st.bst_environ l stmt) ==>
+                  (bir_exec_stmt p stmt st = (NONE, bir_exec_stmt_jmp_to_label p l st))``,
+
+Cases_on `stmt` >>
+SIMP_TAC std_ss [bir_stmt_is_jmp_to_label_def, bir_exec_stmt_def,
+  bir_stmtE_is_jmp_to_label_SEM]);
+
+
+val bir_exec_stmt_status_jumped = store_thm ("bir_exec_stmt_status_jumped",
+``!st p stmt l. (st.bst_status <> BST_JumpOutside l) ==>
+                (((bir_exec_stmt_state p stmt st).bst_status = BST_JumpOutside l)) ==>
+                (~(MEM l (bir_labels_of_program p)) /\
+                (bir_stmt_is_jmp_to_label st.bst_environ l stmt))``,
+
+Cases_on `stmt` >| [
+  SIMP_TAC (std_ss++boolSimps.LIFT_COND_ss++holBACore_ss) [bir_exec_stmt_state_REWRS, LET_DEF] >>
+  METIS_TAC[bir_exec_stmtB_status_not_jumped],
+
+  SIMP_TAC std_ss [bir_exec_stmt_state_REWRS, bir_stmt_is_jmp_to_label_def] >>
+  METIS_TAC[bir_exec_stmtE_status_jumped]
+]);
+
+
+val bir_exec_step_status_jumped = store_thm ("bir_exec_step_status_jumped",
+``!st p l. (st.bst_status <> BST_JumpOutside l) ==>
+           (((bir_exec_step_state p st).bst_status = BST_JumpOutside l)) ==>
+
+                (~(MEM l (bir_labels_of_program p)) /\
+                ((?stmt. (bir_get_current_statement p st.bst_pc = SOME stmt) /\
+                         (bir_stmt_is_jmp_to_label st.bst_environ l stmt))))``,
+
+REPEAT GEN_TAC >>
+SIMP_TAC (std_ss++boolSimps.LIFT_COND_ss) [bir_exec_step_state_def, bir_exec_step_def] >>
+CASE_TAC >> (
+  ASM_SIMP_TAC (std_ss++holBACore_ss) [bir_state_set_failed_def, GSYM bir_exec_stmt_state_def]
+) >>
+METIS_TAC[bir_exec_stmt_status_jumped]);
+
+
+
+
+(*****************************)
+(* Status AssumptionViolated *)
+(*****************************)
+
+
+val bir_exec_stmtB_status_assumption = store_thm ("bir_exec_stmtB_status_assumption",
+``!st stmt. (st.bst_status <> BST_AssumptionViolated) ==>
+            ((bir_exec_stmtB_state stmt st).bst_status = BST_AssumptionViolated) ==>
+            (?e. (stmt = BStmt_Assume e) /\ (bir_eval_exp e st.bst_environ = BVal_Imm (Imm1 0w)))``,
+
+Cases_on `stmt` >> (
+  ASM_SIMP_TAC (std_ss++holBACore_ss) [bir_exec_stmtB_state_REWRS, LET_DEF,
+    bir_exec_stmt_declare_def, bir_exec_stmt_assume_def,
+    bir_exec_stmt_assign_def, bir_exec_stmt_assert_def,
+    bir_exec_stmt_observe_state_def, bir_state_set_failed_def] >>
+  REPEAT GEN_TAC >>
+  REPEAT CASE_TAC >>
+  FULL_SIMP_TAC (std_ss++holBACore_ss) []
+));
+
+
+val bir_exec_stmtE_status_not_assumption = store_thm ("bir_exec_stmtE_status_not_assumption",
+``!st p stmt. (st.bst_status <> BST_AssumptionViolated) ==>
+              ~((bir_exec_stmtE p stmt st).bst_status = BST_AssumptionViolated)``,
+
+Cases_on `stmt` >> (
+  ASM_SIMP_TAC (std_ss++holBACore_ss) [bir_exec_stmtE_def,
+    bir_exec_stmt_jmp_def, bir_state_set_failed_def, bir_exec_stmt_jmp_to_label_def,
+    bir_exec_stmt_cjmp_def, bir_exec_stmt_halt_def, bir_stmtE_is_jmp_to_label_REWRS] >>
+  REPEAT GEN_TAC >>
+  REPEAT CASE_TAC >>
+  FULL_SIMP_TAC (std_ss++holBACore_ss) []
+));
+
+
+val bir_exec_stmt_status_assumption = store_thm ("bir_exec_stmt_status_assumption",
+``!st p stmt. (st.bst_status <> BST_AssumptionViolated) ==>
+              (((bir_exec_stmt_state p stmt st).bst_status = BST_AssumptionViolated)) ==>
+              (?e. (stmt = BStmtB (BStmt_Assume e)) /\ (bir_eval_exp e st.bst_environ = BVal_Imm (Imm1 0w)))``,
+
+Cases_on `stmt` >| [
+  SIMP_TAC (std_ss++boolSimps.LIFT_COND_ss++holBACore_ss) [
+    bir_exec_stmt_state_REWRS, LET_DEF] >>
+  METIS_TAC[bir_exec_stmtB_status_assumption],
+
+  SIMP_TAC (std_ss++holBACore_ss) [bir_exec_stmt_state_REWRS] >>
+  METIS_TAC[bir_exec_stmtE_status_not_assumption]
+]);
+
+
+val bir_exec_step_status_assumption = store_thm ("bir_exec_step_status_assumption",
+``!st p. (st.bst_status <> BST_AssumptionViolated) ==>
+         ((bir_exec_step_state p st).bst_status = BST_AssumptionViolated) ==>
+         (?e. (bir_get_current_statement p st.bst_pc = SOME (BStmtB (BStmt_Assume e))) /\
+              (bir_eval_exp e st.bst_environ = BVal_Imm (Imm1 0w)))``,
+
+REPEAT GEN_TAC >>
+SIMP_TAC (std_ss++boolSimps.LIFT_COND_ss) [bir_exec_step_state_def, bir_exec_step_def] >>
+CASE_TAC >> (
+  ASM_SIMP_TAC (std_ss++holBACore_ss) [bir_state_set_failed_def, GSYM bir_exec_stmt_state_def]
+) >>
+METIS_TAC[bir_exec_stmt_status_assumption]);
+
 
 
 val _ = export_theory();
